README.md
@@ -1,9 +1,10 @@
 #Candidate changes:
 
-* add presuppositions to judgments
-* make datatype(s?) w/ language, ctx as a parameter, prove eq
+* make datatype(s?) w/ language, ctx as a parameter, presuppositions as args, prove eq
 
 #TODOs
 
 * fix various warnings (e.g. hint database)
 * make library of better induction schemes
+* prune obsolete lemmas
+* determine minimal presuppositions needed in proof tree 
